dataLang support for word-at-a-time strings
This adds a dataLang primitive for initializing strings and lowers it to
a sequence of _word_ writes with a precomputed pointer, resulting in
substantially fewer instructions than the previous lowering using byte
writes (on x64, 2 per 8 bytes instead of 56 per 8 bytes).  Modifies the
memory proofs to allow for writing whole strings at once, replaces
write_bytes with a translatable version, and adds plumbing to support
our first endian-specific transformation.

compiler/backend/backendComputeLib.sml
@@ -417,6 +417,13 @@ val add_backend_compset = computeLib.extend_compset
     ,data_to_wordTheory.encode_header_def
     ,data_to_wordTheory.list_Seq_def
     ,data_to_wordTheory.StoreEach_def
+    ,data_to_wordTheory.StoreEachWord_def
+    ,data_to_wordTheory.set_byte_exec_def
+    ,numLib.SUC_RULE data_to_wordTheory.bytes_to_word_exec_def
+    ,byteTheory.byte_index_def
+    ,data_to_wordTheory.write_bytes_def
+    ,data_to_wordTheory.byte_len_def
+    ,data_to_wordTheory.prepare_data_conf_def
     ,data_to_wordTheory.small_shift_length_def
     ,data_to_wordTheory.shift_length_def
     ,data_to_wordTheory.max_heap_limit_def
@@ -728,6 +735,7 @@ val add_backend_compset = computeLib.extend_compset
     ,word_to_stackTheory.write_bitmap_def
     ,word_to_stackTheory.insert_bitmap_def
     ,word_to_stackTheory.wLive_def
+    ,word_to_stackTheory.static_read_def
     ,word_to_stackTheory.SeqStackFree_def
     ,word_to_stackTheory.stack_arg_count_def
     ,word_to_stackTheory.stack_free_def
